composition of upper phases doesn't need a simulation relation,
because at the toplevel, memory doesn't change (even though some
phases may use stackalloc to temporarily introduce more memory,
which will have to show up inside their private simulation relations).
So if we don't include locals in the postconditions, the same
postcondition holds for source and target language execution,
and we don't need a simulation relation to translate postconditions,
and composition of compiler phase correctness is simple.

compiler/src/compiler/UpperPipeline.v
@@ -32,38 +32,34 @@ Section WithWordAndMem.
           (trace -> mem -> Locals -> MetricLog -> Prop) -> Prop
   }.
 
-  Definition relation(L1 L2: Lang): Type := bool ->
-    L1.(Env) -> L1.(Cmd) -> trace -> mem -> L1.(Locals) -> MetricLog ->
-    L2.(Env) -> L2.(Cmd) -> trace -> mem -> L2.(Locals) -> MetricLog -> Prop.
+  Definition phase_correct{L1 L2: Lang}(compile: L1.(Env) -> option L2.(Env)): Prop :=
+    forall functions1 functions2 f_entry_name fbody1,
+      compile functions1 = Some functions2 ->
+      map.get functions1 f_entry_name = Some (nil, nil, fbody1) ->
+      exists fbody2,
+        map.get functions2 f_entry_name = Some (nil, nil, fbody2) /\
+        forall t m mc post, L1.(Exec) functions1 fbody1 t m map.empty mc (fun t' m' l' mc' => post t' m') ->
+                            L2.(Exec) functions2 fbody2 t m map.empty mc (fun t' m' l' mc' => post t' m').
 
-  Definition simulation{L1 L2: Lang}(R: relation L1 L2) :=
-    forall (e1: L1.(Env)) (e2: L2.(Env)) (c1: L1.(Cmd)) (c2: L2.(Cmd))
-           (P1: trace -> mem -> L1.(Locals) -> MetricLog -> Prop)
-           (P2: trace -> mem -> L2.(Locals) -> MetricLog -> Prop),
-      (forall t1 m1 l1 mc1 t2 m2 l2 mc2, R true e1 c1 t1 m1 l1 mc1 e2 c2 t2 m2 l2 mc2 ->
-                                         P1 t1 m1 l1 mc1 -> P2 t2 m2 l2 mc2) ->
-      (forall t1 m1 l1 mc1 t2 m2 l2 mc2, R false e1 c1 t1 m1 l1 mc1 e2 c2 t2 m2 l2 mc2 ->
-                                         L1.(Exec) e1 c1 t1 m1 l1 mc1 P1 ->
-                                         L2.(Exec) e2 c2 t2 m2 l2 mc2 P2).
+  Definition compose_phases{A B C: Type}(phase1: A -> option B)(phase2: B -> option C)(a: A) :=
+    match phase1 a with
+    | Some b => phase2 b
+    | None => None
+    end.
 
-  Definition compose_related{L1 L2 L3: Lang}(R12: relation L1 L2)(R23: relation L2 L3): relation L1 L3 :=
-    fun done e1 c1 t1 m1 l1 mc1 e3 c3 t3 m3 l3 mc3 =>
-      exists e2 c2 t2 m2 l2 mc2, R12 done e1 c1 t1 m1 l1 mc1 e2 c2 t2 m2 l2 mc2 /\
-                                 R23 done e2 c2 t2 m2 l2 mc2 e3 c3 t3 m3 l3 mc3.
-
-  Lemma compose_simulation{L1 L2 L3: Lang}{R12: relation L1 L2}{R23: relation L2 L3}
-        (S12: simulation R12)(S23: simulation R23): simulation (compose_related R12 R23).
+  Lemma compose_phases_correct{L1 L2 L3: Lang}
+        (compile12: L1.(Env) -> option L2.(Env))
+        (compile23: L2.(Env) -> option L3.(Env)):
+    phase_correct compile12 -> phase_correct compile23 -> phase_correct (compose_phases compile12 compile23).
   Proof.
-    unfold simulation, compose_related in *.
-    intros e1 e3 c1 c3 P1 P3 W t1 m1 l1 mc1 t3 m3 l3 mc3 R13 Ex1.
-    simp.
-    eapply S23. 2: eassumption. 2: {
-      eapply S12 with (P2 := (fun t2' m2' l2' mc2' => exists t1' m1' l1' mc1',
-                                  R12 true e1 c1 t1' m1' l1' mc1' e2 c2 t2' m2' l2' mc2' /\
-                                  P1 t1' m1' l1' mc1')).
-      3: eassumption. 2: eassumption. clear. eauto 10.
-    }
-    cbv beta. clear -W. intros. simp. eauto 10.
+    unfold phase_correct, compose_phases. intros C12 C23. intros *. intros ? G1. simp.
+    specialize C12 with (1 := E) (2 := G1). simp.
+    specialize C23 with (1 := H) (2 := C12p0). simp.
+    eexists. split. 1: eassumption.
+    intros *. intro Ex1.
+    specialize C12p1 with (1 := Ex1).
+    specialize C23p1 with (1 := C12p1).
+    exact C23p1.
   Qed.
 
   Section WithMoreParams.
@@ -133,38 +129,24 @@ Section WithWordAndMem.
       eapply intersect; eassumption.
     Qed.
 
-    Definition flattenPhase(prog: SrcLang.(Env)): option FlatLangStr.(Env) :=
-      flatten_functions prog.
-    Definition renamePhase(prog: FlatLangStr.(Env)): option FlatLangZ.(Env) :=
-      rename_functions prog.
-    Definition spillingPhase(prog: FlatLangZ.(Env)): option FlatLangZ.(Env) :=
-      spill_functions prog.
-
-    Definition composePhases{A B C: Type}(phase1: A -> option B)(phase2: B -> option C)(a: A) :=
-      match phase1 a with
-      | Some b => phase2 b
-      | None => None
-      end.
-
-    Definition composedCompileEnv: SrcLang.(Env) -> option FlatLangZ.(Env) :=
-      (composePhases flattenPhase
-      (composePhases renamePhase
-                     spillingPhase)).
-
-    Definition flattening_related: relation SrcLang FlatLangStr :=
-      fun done e1 c1 t1 m1 l1 mc1 e2 c2 t2 m2 l2 mc2 =>
-        ExprImp2FlatImp c1 = c2 /\
-        flatten_functions e1 = Some e2 /\
-        t1 = t2 /\
-        m1 = m2 /\
-        (done = false -> l1 = map.empty /\ l2 = map.empty /\ mc1 = mc2).
-
-    Lemma flattening_sim: simulation flattening_related.
+    Lemma flattening_correct: @phase_correct SrcLang FlatLangStr flatten_functions.
     Proof.
-      unfold simulation, flattening_related, ExprImp2FlatImp. intros.
-      simp. specialize (H0p2 eq_refl). simp.
+      unfold phase_correct. intros.
+
+      pose proof H as GF.
+      unfold flatten_functions in GF.
+      eapply map.map_all_values_fw in GF. 5: eassumption. 2-4: typeclasses eauto.
+      simp. unfold flatten_function in GFp0.
+      (* simp would also unfold freshNameGenState *)
+      apply Option.eq_of_eq_Some in GFp0. destruct v2 as ((? & ?) & ?).
+      eapply pair_equal_spec in GFp0. destruct GFp0 as (GFp0 & ?).
+      eapply pair_equal_spec in GFp0. destruct GFp0 as (GFp0 & ?).
+      subst.
+
+      eexists. split. 1: eassumption.
+      intros.
       eapply FlatImp.exec.weaken.
-      - eapply @flattenStmt_correct_aux with (eH := e1).
+      - eapply @flattenStmt_correct_aux.
         + econstructor; try typeclasses eauto.
         + eassumption.
         + eassumption.
@@ -176,123 +158,47 @@ Section WithWordAndMem.
         + intros x k A. rewrite map.get_empty in A. discriminate.
         + unfold map.undef_on, map.agree_on. intros. reflexivity.
         + eapply freshNameGenState_disjoint.
-      - simpl. intros. simp. eapply H. 2: eassumption. simpl. intuition (discriminate || eauto).
+      - simpl. intros. simp. assumption.
     Qed.
 
-    Definition renaming_related: relation FlatLangStr FlatLangZ :=
-      fun done e1 c1 t1 m1 l1 mc1 e2 c2 t2 m2 l2 mc2 =>
-      RegRename.envs_related e1 e2 /\
-      (exists r' av', RegRename.rename map.empty c1 lowest_available_impvar = Some (r', c2, av')) /\
-      t1 = t2 /\
-      m1 = m2 /\
-      (done = false -> l1 = map.empty /\ l2 = map.empty /\ mc1 = mc2).
-
-    Lemma renaming_sim: simulation renaming_related.
+    Lemma renaming_correct: @phase_correct FlatLangStr FlatLangZ rename_functions.
     Proof.
-      unfold simulation, renaming_related. intros.
-      simp. specialize (H0p3 eq_refl). simp.
-      pose proof H0p1 as A.
-      apply rename_props in A;
-        [|eapply map.empty_injective|eapply dom_bound_empty].
-      simp.
-      eapply FlatImp.exec.weaken.
-      - eapply rename_correct with (ext_spec0 := ext_spec).
-        1: eassumption.
-        1: eassumption.
-        3: {
-          eapply Ap2. eapply TestLemmas.extends_refl.
-        }
-        1: eassumption.
-        1: eassumption.
-        unfold states_compat. intros *. intro B.
-        erewrite map.get_empty in B. discriminate.
-      - simpl. intros. simp.
-        eapply H. 2: eassumption. simpl. clear H. intuition (discriminate || eauto).
-    Qed.
+      unfold phase_correct. intros.
 
-    Axiom TODO: False.
-
-    Definition spilling_related: relation FlatLangZ FlatLangZ :=
-      fun done e1 c1 t1 m1 l1 mc1 e2 c2 t2 m2 l2 mc2 =>
-      c2 = spill_stmt c1 /\
-      exists maxvar (fpval: word),
-        Spilling.envs_related e1 e2 /\
-        Spilling.valid_vars_src maxvar c1 /\
-        Spilling.related ext_spec maxvar (emp True) fpval t1 m1 l1 t2 m2 l2.
-
-    Lemma spilling_sim: simulation spilling_related.
-    Proof.
-      unfold simulation, spilling_related.
-      intros. simp.
-      eapply FlatImp.exec.weaken.
-      - eapply spilling_correct with (ext_spec0 := ext_spec); eassumption.
-      - cbv beta. intros. simp. eapply H. 2: eassumption. simpl.
-        eauto 10.
-    Qed.
-
-    Definition upper_related: relation SrcLang FlatLangZ :=
-      (compose_related flattening_related
-      (compose_related renaming_related
-                       spilling_related)).
-
-    Lemma sim: simulation upper_related.
-    Proof.
-      exact (compose_simulation flattening_sim
-            (compose_simulation renaming_sim
-                                spilling_sim)).
-    Qed.
-
-    (* Note: spilling uses stackalloc to store spilled vars in the memory, so there are some points
-       in execution where the low-level memory differs from the high-level memory, but before and
-       after calling the top-level function the memories are equal, so we can simplify the correctness
-       theorem to this case *)
-
-    Lemma upper_compiler_correct: forall
-        (f_entry_name : string) (fbodyH: Syntax.cmd.cmd)
-        (functionsH: SrcLang.(Env)) (functionsL: FlatLangZ.(Env))
-        t (m: mem) (mc: MetricLog)
-        (post: Semantics.trace -> Semantics.mem -> Prop),
-        ExprImp.valid_funs functionsH ->
-        composedCompileEnv functionsH = Some functionsL ->
-        map.get functionsH f_entry_name = Some (nil, nil, fbodyH) ->
-        Semantics.exec functionsH fbodyH t m map.empty mc (fun t' m' l' mc' => post t' m') ->
-        exists fbodyL, map.get functionsL f_entry_name = Some (nil, nil, fbodyL) /\
-                       FlatImp.exec functionsL fbodyL t m map.empty mc (fun t' m' l' mc' => post t' m').
-    Proof.
-      intros.
-      unfold composedCompileEnv, composePhases in *. simp.
-      rename r into functionsF, r0 into functionsR.
-
-      assert (BW48: bytes_per_word = 4 \/ bytes_per_word = 8). {
-        unfold bytes_per_word.
-        (* PARAMRECORDS doesn't work because the record "Words" is not called "parameters" *)
-        simpl (@Utility.width _).
-        destruct width_cases as [C | C]; rewrite C.
-        + change (Memory.bytes_per_word 32) with 4. auto.
-        + change (Memory.bytes_per_word 64) with 8. auto.
-      }
-
-      pose proof E as GF.
-      unfold flattenPhase, flatten_functions in GF.
-      eapply map.map_all_values_fw in GF. 5: eassumption. 2-4: typeclasses eauto.
-      simp. unfold flatten_function in GFp0.
-      (* simp would also unfold freshNameGenState *)
-      apply Option.eq_of_eq_Some in GFp0. destruct v2 as ((? & ?) & ?).
-      eapply pair_equal_spec in GFp0. destruct GFp0 as (GFp0 & ?).
-      eapply pair_equal_spec in GFp0. destruct GFp0 as (GFp0 & ?).
-      subst.
-
-      pose proof E0 as GR.
-      unfold renamePhase, rename_functions in GR.
+      pose proof H as GR.
+      unfold rename_functions in GR.
       eapply map.map_all_values_fw in GR. 5: eassumption. 2-4: typeclasses eauto.
       simp. unfold rename_fun, rename_binds in GRp0. simp.
 
-      pose proof H0 as GL.
-      unfold spillingPhase in GL.
+      pose proof E as A.
+      apply rename_props in A;
+        [|eapply map.empty_injective|eapply dom_bound_empty].
+      simp.
+      eexists. split. 1: eassumption. intros.
+      eapply FlatImp.exec.weaken.
+      - eapply rename_correct with (ext_spec0 := ext_spec).
+        2: eassumption.
+        { unfold envs_related. intros *. intro G.
+          eapply map.map_all_values_fw. 5: exact G. 4: eassumption. all: typeclasses eauto. }
+        1: eassumption.
+        2: {
+          eapply Ap2. eapply TestLemmas.extends_refl.
+        }
+        1: eassumption.
+        unfold states_compat. intros *. intro B.
+        erewrite map.get_empty in B. discriminate.
+      - simpl. intros. simp. assumption.
+    Qed.
+
+    Lemma spilling_correct: @phase_correct FlatLangZ FlatLangZ spill_functions.
+    Proof.
+      unfold phase_correct. intros.
+
+      pose proof H as GL.
       unfold spill_functions in GL.
       eapply map.map_all_values_fw in GL. 5: eassumption. 2-4: typeclasses eauto.
-      unfold spill_fun in GL. simp. eapply Bool.andb_true_iff in E2.
-      destruct E2 as [_ Fs].
+      unfold spill_fun in GL. simp. eapply Bool.andb_true_iff in E.
+      destruct E as [_ Fs].
       eapply forallb_vars_stmt_correct in Fs. 2: {
         intros x. split; intros F.
         - rewrite ?Z.ltb_lt in F. exact F.
@@ -304,7 +210,7 @@ Section WithWordAndMem.
         - apply  Bool.andb_true_iff. rewrite ?Z.ltb_lt. assumption.
       }
 
-      eexists. split. 1: exact GLp1.
+      eexists. split. 1: eassumption. intros.
 
       unfold spill_fbody.
       eapply FlatImp.exec.stackalloc. {
@@ -313,22 +219,23 @@ Section WithWordAndMem.
       }
       intros *. intros Ab Sp.
 
-      pose proof sim as Sim. unfold simulation, Exec, SrcLang, FlatLangZ in Sim.
-      cbn in Sim. eapply Sim; clear Sim. 3: eassumption.
+      assert (BW48: bytes_per_word = 4 \/ bytes_per_word = 8). {
+        unfold bytes_per_word.
+        (* PARAMRECORDS doesn't work because the record "Words" is not called "parameters" *)
+        simpl (@Utility.width _).
+        destruct width_cases as [C | C]; rewrite C.
+        + change (Memory.bytes_per_word 32) with 4. auto.
+        + change (Memory.bytes_per_word 64) with 8. auto.
+      }
 
-      2: { (* upper_related holds initially: *)
-        unfold upper_related, compose_related, flattening_related, renaming_related, spilling_related. cbn.
-        do 6 eexists. ssplit. all: eauto 3.
-        do 6 eexists. ssplit. all: eauto 3.
-        { unfold envs_related. intros.
-          eapply map.map_all_values_fw. 5: eassumption. 4: eassumption. all: typeclasses eauto. }
-        do 2 eexists. ssplit.
+      eapply FlatImp.exec.weaken.
+      - eapply spilling_correct with (ext_spec0 := ext_spec). 2: eassumption.
         { unfold Spilling.envs_related. intros *. intro G.
-          pose proof H0 as GL'.
-          unfold spillingPhase, spill_functions in GL'.
+          pose proof H as GL'.
+          unfold spill_functions in GL'.
           eapply map.map_all_values_fw in GL'. 5: exact G. 2-4: typeclasses eauto.
           unfold spill_fun in GL'. simp.
-          eapply Bool.andb_true_iff in E2. destruct E2 as (B1 & B3).
+          eapply Bool.andb_true_iff in E. destruct E as (B1 & B3).
           eapply Bool.andb_true_iff in B1. destruct B1 as (B1 & B2).
           eapply List.forallb_to_Forall in B1. 2: {
             intros x F. rewrite Bool.andb_true_iff in F. rewrite ?Z.ltb_lt in F. exact F.
@@ -382,31 +289,39 @@ Section WithWordAndMem.
           - eapply Nat2Z.inj. rewrite LL. rewrite L. rewrite Z2Nat.id by blia.
             rewrite Z.mul_comm. rewrite Z_div_mult by blia. reflexivity.
         }
-      }
+      - cbv beta. intros. simp.
+        unfold Spilling.related in *. simp.
+        match goal with
+        | H: (_ * _)%sep m' |- _ => rename H into HM
+        end.
+        unfold word_array in HM.
+        seprewrite_in @cast_word_array_to_bytes HM.
+        edestruct ll_mem_to_hl_mem with (mL := m') as (mStack' & HM' & D & Ab'). {
+          simpl in *. (* PARAMRECORDS *) ecancel_assumption.
+        }
+        eexists _, _. ssplit.
+        + match goal with
+          | |- ?G => let T := type of Ab' in replace G with T; [exact Ab'|clear Ab']
+          end.
+          f_equal.
+          rewrite List.length_flat_map with (n := Z.to_nat bytes_per_word).
+          * simpl_addrs. rewrite !Z2Nat.id by blia. simpl in *. (* PARAMRECORDS *) blia.
+          * clear. intros. rewrite HList.tuple.length_to_list. reflexivity.
+        + rewrite sep_emp_r in HM'. apply proj1 in HM'. subst m'. unfold map.split.
+          split. 1: reflexivity. exact D.
+        + assumption.
+    Qed.
 
-      (* low-level post holds at the end: *)
-      cbv beta.
-      unfold upper_related, compose_related, flattening_related, renaming_related, spilling_related,
-             Spilling.related. cbn.
-      intros. simp.
-      match goal with
-      | H: (_ * _)%sep m2 |- _ => rename H into HM2
-      end.
-      unfold word_array in HM2.
-      seprewrite_in @cast_word_array_to_bytes HM2.
-      edestruct ll_mem_to_hl_mem with (mL := m2) as (mStack' & HM2' & D & Ab'). {
-        simpl in *. (* PARAMRECORDS *) ecancel_assumption.
-      }
-      eexists _, _. ssplit.
-      - Search fpval. (* can't prove fpval = a because fpval is existentially quantified in
-                         spilling_related before calling Spilling.related *)
+    Definition upper_compiler :=
+      compose_phases flatten_functions (compose_phases rename_functions spill_functions).
 
-    Abort.
-
-    (* Note: Spilling.related has an "exists stackwords", because after spilling, all commands are
-       always wrapped inside a stackalloc block, but if we make the command just an argument-less
-       function call, we can set stackwords to the empty list and simplify "upper_related" *)
-
+    Lemma upper_compiler_correct: @phase_correct SrcLang FlatLangZ upper_compiler.
+    Proof.
+      unfold upper_compiler.
+      eapply (@compose_phases_correct SrcLang FlatLangStr FlatLangZ). 1: exact flattening_correct.
+      eapply (@compose_phases_correct FlatLangStr FlatLangZ FlatLangZ). 1: exact renaming_correct.
+      exact spilling_correct.
+    Qed.
 
   End WithMoreParams.
 End WithWordAndMem.
